src/semantics.lean
@@ -8,8 +8,8 @@ open dvector
 structure model (L : language.{u}) :=
 (dom : Type u)
 (one : dom)
-(fn : ∀ {n}, L.fn n → dvector dom n → dom)
-(pr : ∀ {n}, L.pr n → dvector dom n → Prop)
+(fn : ∀ {n}, L.fn n → (fin n → dom) → dom)
+(pr : ∀ {n}, L.pr n → (fin n → dom) → Prop)
 
 notation `|`M`|` := model.dom M
 
@@ -17,21 +17,16 @@ variables {L : language.{u}} {M : model L}
 
 instance (M : model L) : inhabited M.dom := ⟨M.one⟩
 
-@[simp] def vecterm.val (e : ℕ → |M|) : ∀ {n} (t : vecterm L n), dvector M.dom (n+1)
-| _ (vecterm.cons a v) := a.val.head :: v.val
-| _ (#x)               := unary (e x)
-| _ (vecterm.const c)  := unary (M.fn c dvector.nil)
-| _ (vecterm.app f v)  := unary (M.fn f v.val)
+@[simp] def term.val (e : ℕ → |M|) : term L → |M|
+| (#x)           := e x
+| (term.app f v) := M.fn f (λ i, (v i).val)
 
-@[simp] def term.val (e : ℕ → |M|) (t : term L) : M.dom := (t.val e).head
-
-@[simp] def formula.val : (ℕ → |M|) → formula L → Prop
-| _ (formula.const c) := M.pr c dvector.nil
-| e (formula.app p v) := M.pr p (v.val e)
-| e (t =̇ u)        := t.val e = u.val e
-| e (p →̇ q)       := p.val e → q.val e
-| e (¬̇p)           := ¬(p.val e)
-| e (∀̇p)           := ∀ d : M.dom, (p.val (d ⌢ e))
+@[simp] def formula.val : ∀ (e : ℕ → |M|), formula L → Prop
+| e (formula.app p v) := M.pr p (λ i, (v i).val e)
+| e (t =̇ u)           := t.val e = u.val e
+| e (p →̇ q)          := p.val e → q.val e
+| e (¬̇p)              := ¬(p.val e)
+| e (∀̇p)              := ∀ d : M.dom, (p.val (d ⌢ e))
 
 notation M` ⊧[`:80 e`] `p :50 := @formula.val _ M e p
 
@@ -41,38 +36,28 @@ infix ` ⊧ `:50 := models
 def modelsth (M : model L) (T : theory L) : Prop := ∀ p, p ∈ T → M ⊧ p
 infix ` ⊧ₜₕ `:50 := modelsth
 
-lemma rew_val_eq : ∀ (s : ℕ → term L) {n} (t : vecterm L n) (e : ℕ → |M|),
+lemma rew_val_eq (s : ℕ → term L) (e : ℕ → |M|) : ∀ (t : term L),
   (t.rew s).val e = t.val (λ n, (s n).val e)
-| _ _ (vecterm.cons a v) _ := by simp[vecterm.rew, rew_val_eq _ a, rew_val_eq _ v]
-| _ _ (#x)               _ := by {simp[vecterm.rew, term.val] }
-| _ _ (vecterm.const c)  _ := rfl 
-| _ _ (vecterm.app f v)  _ := by simp[vecterm.rew, rew_val_eq _ v]
+| (#x)                := by simp
+| (@term.app _ n f v) := by simp[λ i : fin n, rew_val_eq (v i)]
 
-@[simp] lemma pow_val_concat {n} (t : vecterm L n) : ∀ (e : ℕ → |M|) d, (t^1).val (d ⌢ e) = t.val e :=
-by { induction t; simp[concat] at*; simp* }
+@[simp] lemma pow_val_concat (e : ℕ → |M|) (d : |M|) (t : term L) : (t^1).val (d ⌢ e) = t.val e :=
+by simp[term.pow_eq, rew_val_eq]
 
 lemma rew_val_iff : ∀ (s : ℕ → term L) (p : formula L) (e : ℕ → |M|),
   (p.rew s).val e ↔ p.val (λ n, (s n).val e)
-| _ (formula.const c) _ := by simp[formula.rew]
 | _ (formula.app p v) _ := by simp[formula.rew, rew_val_eq]
-| _ (t =̇ u)        _ := by simp[formula.rew, term.val, rew_val_eq]
-| _ (p →̇ q)       _ := by simp[formula.rew, rew_val_iff _ p, rew_val_iff _ q]
-| _ (¬̇p)           _ := by simp[formula.rew, rew_val_iff _ p]
-| s (∀̇p)           e := by { simp[formula.rew, rew_val_iff _ p], refine forall_congr (λ d, _),
-    have : (λ n, (vecterm.val (d ⌢ e) (s^1 $ n)).head) = (d ⌢ λ n, ((s n).val e)),
-    { funext n, cases n; simp[concat, term.val, vecterm.val], exact pow_val_concat _ _ _ },
-    simp[this] }
+| _ (t =̇ u)           _ := by simp[formula.rew, term.val, rew_val_eq]
+| _ (p →̇ q)          _ := by simp[formula.rew, rew_val_iff _ p, rew_val_iff _ q]
+| _ (¬̇p)              _ := by simp[formula.rew, rew_val_iff _ p]
+| s (∀̇p)              e :=
+  by { simp[formula.rew, rew_val_iff _ p], refine forall_congr (λ d, _),
+       have : (λ n, ((s ^ 1) n).val (d ⌢ e) ) = (d ⌢ λ n, ((s n).val e)),
+       { funext n, cases n; simp[concat, term.val, term.val], exact pow_val_concat _ _ _ },
+       simp[this] }
 
-@[simp] lemma pow_val_concat_iff : ∀ (p : formula L) (e : ℕ → |M|) d, (p^1).val (d ⌢ e) = p.val e
-| (formula.const c) _ _ := rfl
-| (formula.app p v) _ _ := by simp
-| (t =̇ u)        _ _ := by simp[term.val]
-| (p →̇ q)       _ _ := by simp[pow_val_concat_iff p, pow_val_concat_iff q]
-| (¬̇p)           _ _ := by simp[pow_val_concat_iff p]
-| (∀̇p)           e d₀ := by {intros, simp, simp[formula.pow_eq, rew_val_iff], apply forall_congr,
-    intros d,
-    have : (λ n, (vecterm.val (d ⌢ d₀ ⌢ e) ((λ x, #(x + 1))^1 $ n)).head) = (d ⌢ e),
-    { ext n, cases n; simp[concat] }, simp[this] }
+@[simp] lemma pow_val_concat_iff : ∀ (p : formula L) (e : ℕ → |M|) d, (p^1).val (d ⌢ e) = p.val e :=
+by simp[formula.pow_eq, rew_val_iff]
 
 private lemma modelsth_sf {T} : M ⊧ₜₕ T → M ⊧ₜₕ ⇑T := λ h p hyp_p e,
 by { rcases hyp_p with ⟨p, hyp_p', rfl⟩, simp[formula.pow_eq, rew_val_iff],
@@ -87,10 +72,17 @@ by simp[formula.and]
 @[simp] lemma models_iff {p q} {e : ℕ → |M|} : (p ↔̇ q).val e ↔ (p.val e ↔ q.val e) :=
 by simp[formula.iff]; exact iff_def.symm
 
-@[simp] lemma models_equals : ∀ {n} (v₁ v₂ : vecterm L n) (e : ℕ → |M|),
-  (v₁ ≡̇ v₂).val e ↔ v₁.val e = v₂.val e
-| 0     t₁ t₂ e := by simp[formula.val]
-| (n+1) (vecterm.cons t₁ v₁) (vecterm.cons t₂ v₂) e := by simp[formula.val, models_equals v₁ v₂]
+@[simp] lemma models_conjunction' {n : ℕ} {P : finitary (formula L) n} {e : ℕ → |M|} :
+  (conjunction' n P).val e ↔ ∀ i, (P i).val e :=
+by { induction n with n IH; simp[formula.top],
+     { intros i, exfalso, exact i.val.not_lt_zero i.property },
+     { simp [IH], split,
+       { rintros ⟨h0, h1⟩, intros i,
+         have : i.val < n ∨ i.val = n := nat.lt_succ_iff_lt_or_eq.mp i.property,
+         cases this,
+         { have := h1 ⟨↑i, this⟩, simp at this, refine this },
+         { simp[←this] at*, refine h0 } },
+       { intros h, refine ⟨h _, λ _, h _⟩ } } }
 
 @[simp] lemma models_pow {p : formula L} {i : ℕ} {e : ℕ → |M| } : (p^i).val e ↔ p.val (λ n, e (n + i)) :=
 by simp[formula.pow_eq, rew_val_iff]
@@ -98,11 +90,10 @@ by simp[formula.pow_eq, rew_val_iff]
 lemma models_subst {p : formula L} {i : ℕ} {t : term L} {e : ℕ → |M| } :
   (p.rew ι[i ⇝ t]).val e ↔ p.val (λ n, if n < i then e n else if i < n then e (n - 1) else t.val e) :=
 by { simp[rew_val_iff],
-     have : (λ (n : ℕ), (vecterm.val e (ι[i ⇝ t] n)).head) =
-     (λ n, if n < i then e n else if i < n then e (n - 1) else t.val e),
+     have : (λ (n : ℕ), term.val e (ι[i ⇝ t] n)) = (λ n, if n < i then e n else if i < n then e (n - 1) else t.val e),
      { funext n,
        have C : n < i ∨ n = i ∨ i < n, exact trichotomous n i,
-       cases C; simp[C],
+       cases C, simp[C],
        cases C; simp[C], simp[asymm C] },
      simp[this] }
 
@@ -114,10 +105,17 @@ by { have := @models_subst _ _ p 0 t e, simp at this,
 
 @[simp] lemma models_subst_1 {p : formula L} {t : term L} {e : ℕ → |M| } :
   (p.rew ι[1 ⇝ t]).val e ↔ p.val (e 0 ⌢ t.val e ⌢ (λ x, e (x + 1))) :=
-by { have := @models_subst _ _ p 1 t e, simp at this,
-     have eqn : (λ n, ite (n < 1) (e n) (ite (1 < n) (e (n - 1)) (vecterm.val e t).head)) =
+by { have := @models_subst _ _ p 1 t e,
+     have eqn : (λ n, ite (n < 1) (e n) (ite (1 < n) (e (n - 1)) (t.val e))) =
        e 0 ⌢ t.val e ⌢ (λ x, e (x + 1)),
      { funext n, cases n; simp[←nat.add_one], cases n; simp }, rw[←eqn], exact this }
+
+lemma nfal_models_iff : ∀ {n} {p : formula L}, M ⊧ nfal p n ↔ M ⊧ p
+| 0     _ := iff.rfl
+| (n+1) p := by { simp[←@nfal_models_iff n p], refine ⟨λ h e, _, λ h e d, h _⟩,
+  have : ((e 0) ⌢ λ x, e (x + 1) )= e, { ext x, cases x; simp[concat] },
+  have := h (λ x, e (x + 1)) (e 0), simp* at* }
+
 
 theorem soundness {T : theory L} : ∀ {p}, T ⊢ p → ∀ {M}, M ⊧ₜₕ T → M ⊧ p := λ p hyp,
 begin
@@ -136,63 +134,60 @@ begin
   { intros M hyp_T e h₁, simp[formula.val], contrapose, exact h₁ },
   case fopl.provable.q1 : T p t
   { intros M hyp_T e h, simp[rew_val_iff] at h ⊢,
-    have : (λ n, (vecterm.val e (ι[0 ⇝ t] n)).head) = (t.val e) ⌢ e,
-    { funext n, cases n; simp[term.val, vecterm.val, concat] },
+    have : (λ n, (ι[0 ⇝ t] n).val e) = (t.val e) ⌢ e,
+    { funext n, cases n; simp[term.val, term.val, concat] },
     rw this, exact h _ },
   case fopl.provable.q2 : T p q
   { intros M hyp_T e h₁ h₂ d, exact (h₁ d) (h₂ d) },
   case fopl.provable.q3 : T p
   { intros M hyp_T e h d, simp, exact h },
-  case fopl.provable.e1 : T t
-  { intros M hyp_T e, simp[formula.val] },
-  case fopl.provable.e2 : T t₁ t₂
-  { intros M hyp_T e, simp[formula.val], refine eq.symm },
-  case fopl.provable.e3 : T t₁ t₂ t₃
-  { intros M hyp_T e, simp[formula.val], refine eq.trans },
-  case fopl.provable.e4 : T n t₁ t₂ f
-  { intros M hyp_T e, simp[formula.val], refine λ eqn, (by simp[eqn]) },
-  case fopl.provable.e5 : T n t₁ t₂ f
-  { intros M hyp_T e, simp[formula.val], refine λ eqn, (by simp[eqn]) },
+  case fopl.provable.e1 : T
+  { intros M hyp_T e t, simp[formula.val] },
+  case fopl.provable.e2 : T
+  { intros M hyp_T e t₁ t₂, simp[formula.val], refine eq.symm },
+  case fopl.provable.e3 : T
+  { intros M hyp_T e t₁ t₂ t₃, simp[formula.val], refine eq.trans },
+  case fopl.provable.e4 : T n f
+  { simp[eq_axiom4, nfal_models_iff], intros M hyp_T e,
+    simp, intros h, simp[h] },
+  case fopl.provable.e5 : T n f
+  { simp[eq_axiom5, nfal_models_iff], intros M hyp_T e,
+    simp, intros h, simp[h] },
 end
 
 theorem model_consistent {T : theory L} : M ⊧ₜₕ T → theory.consistent T :=
 by { contrapose, simp[theory.consistent], intros p hp₁ hp₂ hyp,
      exact soundness hp₂ hyp (λ _, (default M.dom)) (soundness hp₁ hyp (λ _, (default M.dom))) }
 
-lemma eval_eq : ∀ {n} {v : vecterm L n} {e₁ e₂ : ℕ → |M|},
-  (∀ n, n < v.arity → e₁ n = e₂ n) → v.val e₁ = v.val e₂
-| (n+1) (vecterm.cons t v) e₁ e₂ a := by { simp[vecterm.arity] at *,
-    refine ⟨eval_eq (λ n h, a _ (or.inl h)), eval_eq (λ n h, a _ (or.inr h))⟩ }
-| _     (#n)               _  _  a := by { simp[vecterm.arity] at *, refine a _ _, simp }
-| _     (vecterm.const c)  _  _  a := by simp
-| _     (vecterm.app f v)  e₁ e₂ a := by { simp[vecterm.arity] at *, 
-    simp[eval_eq a] } 
+lemma eval_eq : ∀ {t : term L} {e₁ e₂ : ℕ → |M|},
+  (∀ n, n < t.arity → e₁ n = e₂ n) → t.val e₁ = t.val e₂
+| (#n)               _  _  eqs := by simp at *; refine eqs _ _; simp
+| (@term.app _ n f v)  e₁ e₂ eqs := by { simp at *, congr, funext i, refine @eval_eq (v i) _ _ (λ n eqn, _),
+  have : (v i).arity ≤ finitary.Max 0 (λ i, (v i).arity), from finitary.Max_le 0 (λ i, (v i).arity) i,
+  refine eqs n (lt_of_lt_of_le eqn this) } 
 
 lemma eval_iff : ∀ {p : formula L} {e₁ e₂ : ℕ → |M|},
   (∀ n, n < p.arity → e₁ n = e₂ n) → (M ⊧[e₁] p ↔ M ⊧[e₂] p)
-| (formula.const _) _  _  _ := by simp* at *
-| (formula.app p v) e₁ e₂ a := by { simp[sentence, formula.arity] at*, simp[eval_eq a] }
-| (t =̇ u)        e₁ e₂ a := by { simp[sentence, formula.arity] at*,
-  simp[eval_eq (λ n h, a _ (or.inl h)), eval_eq (λ n h, a _ (or.inr h))] }
-| (p →̇ q)       e₁ e₂ a := by { simp[sentence, formula.arity] at*,
-    simp[eval_iff (λ n h, a _ (or.inl h)), eval_iff (λ n h, a _ (or.inr h))] }
-| (¬̇p)           e₁ e₂ a := by { simp[sentence, formula.arity] at*,
-    simp[eval_iff a] }
-| (∀̇p)           e₁ e₂ a := by { simp[sentence, formula.arity] at*,
+| (@formula.app _ n p v) e₁ e₂ eqs := by { simp[sentence] at*,
+    suffices : (λ i, term.val e₁ (v i)) = (λ i, term.val e₂ (v i)), { simp[this] },
+    funext i, refine @eval_eq _ M (v i) _ _ (λ n eqn, eqs n _),
+    have : (v i).arity ≤ finitary.Max 0 (λ i, (v i).arity), from finitary.Max_le 0 (λ i, (v i).arity) i,
+    refine (lt_of_lt_of_le eqn this) }
+| (t =̇ u)                e₁ e₂ eqs := by { simp[sentence, formula.arity] at*,
+    simp[eval_eq (λ n h, eqs _ (or.inl h)), eval_eq (λ n h, eqs _ (or.inr h))] }
+| (p →̇ q)               e₁ e₂ eqs := by { simp[sentence, formula.arity] at*,
+    simp[eval_iff (λ n h, eqs _ (or.inl h)), eval_iff (λ n h, eqs _ (or.inr h))] }
+| (¬̇p)                   e₁ e₂ eqs := by { simp[sentence, formula.arity] at*,
+    simp[eval_iff eqs] }
+| (∀̇p)                   e₁ e₂ eqs := by { simp[sentence, formula.arity] at*,
     have : ∀ (d : |M|), p.val (d ⌢ e₁) ↔ p.val (d ⌢ e₂),
     { intros d, refine eval_iff (λ n eqn, _),
-      cases n; simp[concat], refine a _ (nat.lt_sub_right_of_add_lt eqn) },
+      cases n; simp[concat], refine eqs _ (nat.lt_sub_right_of_add_lt eqn) },
     exact forall_congr this }
 
 lemma eval_sentence_iff {p : formula L} {e : ℕ → |M|} (a : sentence p) : M ⊧[e] p ↔ M ⊧ p :=
 ⟨λ h e, by { refine (eval_iff $ λ n h, _).1 h, exfalso,
  simp[sentence] at*, rw[a] at h, exact nat.not_lt_zero n h},
  λ h, h e⟩
-
-lemma nfal_models_iff : ∀ {n} {p : formula L}, M ⊧ p ↔ M ⊧ nfal p n
-| 0     _ := iff.rfl
-| (n+1) p := by { simp[@nfal_models_iff n p], refine ⟨λ h e d, h _, λ h e, _⟩,
-  have : ((e 0) ⌢ λ x, e (x + 1) )= e, { ext x, cases x; simp[concat] },
-  have := h (λ x, e (x + 1)) (e 0), simp* at * }
 
 end fopl
